IrisCore/Misc.thy
@@ -6,33 +6,47 @@ definition map_heap :: "('l\<rightharpoonup>'v::ofe) \<Rightarrow> ('l\<times>'v
   "map_heap h f a = folding_on.F f a {(l,v) |l v. h l = Some v}"
 
 definition sep_map_heap :: "('l\<rightharpoonup>'v::ofe) \<Rightarrow> ('l\<times>'v\<Rightarrow>iprop) \<Rightarrow> iprop" where
-  "sep_map_heap h f = map_heap h (\<lambda>lv a. a \<^emph> f lv) (\<upharpoonleft>True)"
+  "sep_map_heap h f = map_heap h (\<lambda>lv a. a \<^emph> f lv) upred_emp"
 
 definition sep_map_set :: "('b\<Rightarrow>iprop) \<Rightarrow> 'b set \<Rightarrow> iprop" where
-  "sep_map_set f s = folding_on.F (\<lambda>x a. a \<^emph> f x) (\<upharpoonleft>True) s"
+  "sep_map_set f s = folding_on.F (\<lambda>x a. a \<^emph> f x) upred_emp s"
 
-definition sep_map_fset :: "('b\<Rightarrow>iprop) \<Rightarrow> 'b fset \<Rightarrow> iprop" where
-  "sep_map_fset f s = folding_on.F (\<lambda>x a. a \<^emph> f x) (\<upharpoonleft>True) (fset s)"
+abbreviation sep_emp_fold_list :: "iprop list \<Rightarrow> iprop" ("[\<^emph>\<^sub>l] _") where
+  "sep_emp_fold_list l \<equiv> foldl (\<^emph>) upred_emp l"
+
+abbreviation sep_fold_list :: "iprop \<Rightarrow> iprop list \<Rightarrow> iprop" ("[\<^emph>\<^sub>l _] _") where 
+  "sep_fold_list acc l \<equiv> foldl (\<^emph>) acc l"
   
+definition sep_fold_fset :: "('a \<Rightarrow> iprop) \<Rightarrow> 'a fset \<Rightarrow> iprop \<Rightarrow> iprop" ("[\<^emph>\<^sub>f] _ _ _") where
+  "sep_fold_fset f s acc = ffold (\<lambda>x a. a \<^emph> f x) acc s"
+
+abbreviation sep_map_fset :: "('b\<Rightarrow>iprop) \<Rightarrow> 'b fset \<Rightarrow> iprop" ("[\<^emph>\<^sub>m] _ _") where
+  "sep_map_fset f s \<equiv> sep_fold_fset f s upred_emp"
+
 abbreviation sep_map_fmdom :: "('b\<Rightarrow>iprop) \<Rightarrow> ('b,'a) fmap \<Rightarrow> iprop" where
   "sep_map_fmdom f m \<equiv> sep_map_fset f (fmdom m)"
-  
+
+lemma sep_comp_fun_commute: "comp_fun_commute (\<^emph>)"
+  apply standard apply (simp add: comp_def)
+  by (metis upred_sep_assoc_eq upred_sep_comm)
+
+lemma sep_P_comp_fun_commute: "comp_fun_commute (\<lambda>x a. a \<^emph> P x)"
+  apply standard apply (simp add: comp_def comp_fun_commute_def upred_sep_comm)
+  by (metis (no_types, opaque_lifting) upred_sep_assoc_eq upred_sep_comm)
+
 lemma sep_map_dom_delete: "fmlookup m i = Some x \<Longrightarrow> 
   sep_map_fmdom P m = P i \<^emph> sep_map_fmdom P (fmdrop i m)"
 unfolding sep_map_set_def
 proof -
   assume "fmlookup m i = Some x"
   then have i_fin: "i |\<in>| fmdom m" by (rule fmdomI)
-  then have i_in: "i \<in> fset (fmdom m)" by (simp add: fmember.rep_eq)
-  have fold_on: "folding_on UNIV (\<lambda>x a. a \<^emph> P x)" by standard (auto simp: comp_def upred_sep_comm2_eq)
-  have "finite (fset (fmdom m))" by simp
   have drop_minus: "fmdom (fmdrop i m) = (fmdom m |-| {|i|})" by simp
-  have "folding_on.F (\<lambda>x a. a \<^emph> P x) (\<upharpoonleft>True) (fset (fmdom m)) =
-    folding_on.F (\<lambda>x a. a \<^emph> P x) (\<upharpoonleft>True) (fset (fmdom m |-| {|i|})) \<^emph> (P i)"
-  using folding_on.remove[OF fold_on _ \<open>finite (fset (fmdom m))\<close> i_in, simplified] by auto
-  with drop_minus have "folding_on.F (\<lambda>x a. a \<^emph> P x) (\<upharpoonleft>True) (fset (fmdom m)) =
-    folding_on.F (\<lambda>x a. a \<^emph> P x) (\<upharpoonleft>True) (fset (fmdom (fmdrop i m))) \<^emph> (P i)" by simp
+  have "ffold (\<lambda>x a. a \<^emph> P x) upred_emp (fmdom m) =
+    ffold (\<lambda>x a. a \<^emph> P x) upred_emp (fmdom m |-| {|i|}) \<^emph> (P i)"
+  using comp_fun_commute.ffold_rec[OF sep_P_comp_fun_commute i_fin] .
+  with drop_minus have "ffold (\<lambda>x a. a \<^emph> P x) (\<upharpoonleft>True) (fmdom m) =
+    ffold (\<lambda>x a. a \<^emph> P x) upred_emp (fmdom (fmdrop i m)) \<^emph> (P i)" by simp
   then show "sep_map_fmdom P m = P i \<^emph> sep_map_fmdom P (fmdrop i m)" 
-    using sep_map_fset_def upred_sep_comm by metis
-qed    
+    unfolding sep_fold_fset_def using upred_sep_comm by auto
+qed
 end
